parse client hello progress

src/tls13crypto.rs
@@ -625,6 +625,7 @@ pub struct Algorithms {
     pub(crate) zero_rtt: bool,
 }
 
+#[hax_lib::attributes]
 impl Algorithms {
     /// Create a new [`Algorithms`] object for the TLS 1.3 ciphersuite.
     pub const fn new(
@@ -712,6 +713,10 @@ impl Algorithms {
     }
 
     /// Check the ciphersuite in `bytes` against this ciphersuite.
+    #[hax_lib::ensures(|result| match result {
+                                    Result::Ok(len) => bytes.len() >= len && len < 65538,
+                                    _ => true
+                                })]
     pub(crate) fn check(&self, bytes: &[U8]) -> Result<usize, TLSError> {
         let len = length_u16_encoded(bytes)?;
         let cs = self.ciphersuite()?;
